& (1) && \alpha \rightarrow 0 & \text{(assumption)}\\
& (2) && \beta & \text{(assumption)}\\
& (3) && \phi \rightarrow ((\phi \rightarrow \psi) \rightarrow \psi) & \text{(MP, R1b, R1b)}\\
& (4) && ((\phi \rightarrow \phi) \rightarrow \psi) \rightarrow (0 \rightarrow \psi) & \text{(MP, R5a, R1a)}\\
& (5) && (0 \rightarrow \phi) \rightarrow (\alpha \rightarrow \phi) & \text{(MP, 1, R1a)}\\
& (6) && (\beta \rightarrow \phi) \rightarrow \phi & \text{(MP, 2, 3)}\\
& (7) && 0 \rightarrow \beta & \text{(MP, 6, 4)}\\
& (8) && \alpha \rightarrow \beta & \text{(MP, 7, 5)}
