& (1) && \alpha & \text{(assumption)}\\
& (2) && \beta \rightarrow 0 & \text{(assumption)}\\
& (3) && (((\phi \rightarrow \psi) \rightarrow (\chi \rightarrow \psi)) \rightarrow \omega) \rightarrow ((\chi \rightarrow \phi) \rightarrow \omega) & \text{(MP, R1a, R1a)}\\
& (4) && \phi \rightarrow ((\phi \rightarrow \psi) \rightarrow \psi) & \text{(MP, R1b, R1b)}\\
& (5) && ((\beta \rightarrow 0) \rightarrow \phi) \rightarrow \phi & \text{(MP, 2, 4)}\\
& (6) && (\alpha \rightarrow \phi) \rightarrow \phi & \text{(MP, 1, 4)}\\
& (7) && (\phi \rightarrow \beta) \rightarrow (\phi \rightarrow 0) & \text{(MP, 5, 3)}\\
& (8) && (\alpha \rightarrow \beta) \rightarrow 0 & \text{(MP, 6, 7)}
