& (1) && (\alpha \rightarrow \beta) \lor 0 \rightarrow 0 & \text{(assumption)}\\
& (2) && (\phi \lor \psi \rightarrow \chi) \rightarrow (\phi \rightarrow \chi) & \text{(MP, R2, R1a)}\\
& (3) && (\alpha \rightarrow \beta) \rightarrow 0 & \text{(MP, 1, 2)}\\
& (4) && (0 \rightarrow \phi) \rightarrow ((\alpha \rightarrow \beta) \rightarrow \phi) & \text{(MP, 3, R1a)}\\
& (5) && (\alpha \rightarrow \beta) \rightarrow (\phi \rightarrow \phi) & \text{(MP, R5a, 4)}\\
& (6) && \beta \rightarrow \alpha & \text{(MP, 5, R1b)}
